$$
42 =
\left(
    \sum_{k=1}^{3} k^2
    - \sqrt{49}
    + \sin(\pi)
\right)
\cdot
\left(
    \prod_{k=1}^{3} k
\right)
\cdot
\frac{
    \displaystyle \int_{0}^{\pi} \sin^2(x)\,dx
    + \ln(e^2)
    - \zeta(0)
}{
    \displaystyle \int_{0}^{\pi} \sin^2(x)\,dx
    + \ln(e^2)
    - \zeta(0)
}

$$
**Summe:**
$$

\sum_{k=1}^{3} k^2 = 1^2 + 2^2 + 3^2 = 1 + 4 + 9 = 14

$$
**Wurzel:**
$$\sqrt{49} = 7$$
**Sinus:**
$$\sin(\pi) = 0$$
**First Block:**
$$\left( 14 - 7 + 0 \right) = 7$$

**Produkt:**
$$\prod_{k=1}^{3} k = 1 \cdot 2 \cdot 3 = 6$$

**Integral:**

$$\int_0^\pi \sin^2(x)\,dx = \frac{\pi}{2}$$
**Logarithmus:**

$$\ln(e^2) = 2$$

**Riemannsche Zeta‑Funktion:**

$$\zeta(0) = -\frac{1}{2}$$

**Zusammensetzen:**

$$\frac{\pi}{2} + 2 - \left(-\frac{1}{2}\right)

= \frac{\pi}{2} + 2 + \frac{1}{2}

= \frac{\pi}{2} + \frac{5}{2}$$

**Zähler = Nenner ->  Bruch = 1.**

$$\frac{A}{A} = 1$$

# Solution:

First Block: 7
Second Block: 6
Bruch: 1

7 x 6 x 1 = 42